examples/grepProgScript.sml
@@ -542,7 +542,8 @@ Theorem print_matching_lines_in_file_spec
   \\ xlet_auto >- xsimpl
   \\ qmatch_asmsub_abbrev_tac`add_stdout fs out`
   \\ imp_res_tac nextFD_ltX
-  \\ imp_res_tac IS_SOME_get_file_content_openFileFS_nextFD \\ rfs[]
+  \\ progress inFS_fname_ALOOKUP_EXISTS
+  \\ progress IS_SOME_get_file_content_openFileFS_nextFD \\ rfs[]
   \\ imp_res_tac STD_streams_nextFD
   \\ rpt(first_x_assum(qspecl_then[`0`,`ReadMode`]strip_assume_tac))
   \\ xlet_auto >- (
@@ -680,32 +681,24 @@ val grep_sem_ind = theorem"grep_sem_ind";
 *)
 
 Theorem grep_sem_file_MAP_FST_infds[simp]
-  `consistentFS fs ⇒ MAP FST (grep_sem_file L ls nm fs).infds = MAP FST fs.infds`
+  `consistentFS fs ⇒ MAP FST (grep_sem_file L nm fs).infds = MAP FST fs.infds`
   (rw[grep_sem_file_def] \\ CASE_TAC \\ simp[] \\ CASE_TAC \\ simp[]
   \\ fs[consistentFS_def] \\ res_tac \\ fs[ALOOKUP_NONE]);
 
 Theorem grep_sem_file_maxFD[simp]
-  `(grep_sem_file L ls nm fs).maxFD = fs.maxFD`
-  (rw[grep_sem_file_def] \\ CASE_TAC \\ simp[]);
+  `consistentFS fs ⇒ (grep_sem_file L nm fs).maxFD = fs.maxFD`
+  (rw[grep_sem_file_def,consistentFS_def] \\ CASE_TAC \\ simp[] \\ res_tac \\
+  CASE_TAC \\ fs[ALOOKUP_NONE]);
 
 Theorem STD_streams_grep_sem_file
-  `consistentFS fs /\ STD_streams fs ⇒ STD_streams (grep_sem_file L fls fn fs)`
+  `consistentFS fs /\ STD_streams fs ⇒ STD_streams (grep_sem_file L fn fs)`
   (rw[grep_sem_file_def,consistentFS_def]
   \\ rpt CASE_TAC \\ simp[STD_streams_add_stderr,STD_streams_add_stdout]
   \\ res_tac >> fs[ALOOKUP_NONE]);
 
-Theorem grep_sem_file_FILTER_File[simp]
-  `grep_sem_file L (FILTER (isFile o FST) ls) = grep_sem_file L ls`
-  (rw[grep_sem_file_def,FUN_EQ_THM,ALOOKUP_FILTER,o_DEF,LAMBDA_PROD]);
-
-Theorem grep_sem_FILTER_File[simp]
-  `∀cl ls. grep_sem cl (FILTER (isFile o FST) ls) = grep_sem cl ls`
-  (ho_match_mp_tac grep_sem_ind
-  \\ rw[grep_sem_def]);
-
 Theorem consistentFS_grep_sem_file[simp]
   `consistentFS fs ⇒
-    consistentFS (grep_sem_file L fls fn fs)`,
+    consistentFS (grep_sem_file L fn fs)`
  (rw[grep_sem_file_def,consistentFS_def]
   \\ rpt CASE_TAC
   \\ fs[up_stdo_files,add_stdo_def] \\
@@ -713,7 +706,7 @@ Theorem consistentFS_grep_sem_file[simp]
 
 Theorem grep_sem_file_lemma
   `consistentFS fs /\ STD_streams fs ⇒
-   let fs' = FOLDL (λa f. grep_sem_file L fls f o a) I ls fs in
+   let fs' = FOLDL (λa f. grep_sem_file L f o a) I ls fs in
      STD_streams fs'∧ consistentFS fs' ∧ (hasFreeFD fs ⇒ hasFreeFD fs') ∧
      FILTER (isFile o FST) fs'.inode_tbl = FILTER (isFile o FST) fs.inode_tbl ∧
      fs'.files = fs.files`
@@ -733,7 +726,7 @@ Theorem grep_sem_file_lemma
 
 Theorem grep_sem_file_lemma'
   `consistentFS fs ⇒
-     consistentFS (FOLDL (λa f. grep_sem_file L fls f o a) I ls fs)`
+     consistentFS (FOLDL (λa f. grep_sem_file L f o a) I ls fs)`
  (simp[]
   \\ qid_spec_tac`fs`
   \\ qid_spec_tac`ls`
@@ -742,19 +735,21 @@ Theorem grep_sem_file_lemma'
 
 Theorem grep_sem_file_with_numchars
   `consistentFS fs ⇒
-   grep_sem_file L file filename (fs with numchars := ns) =
-   grep_sem_file L file filename fs with numchars := ns`
+   grep_sem_file L filename (fs with numchars := ns) =
+   grep_sem_file L filename fs with numchars := ns`
   (rw[grep_sem_file_def,consistentFS_def] \\ CASE_TAC \\ rw[add_stdo_with_numchars]
   \\ CASE_TAC \\ res_tac \\ fs[ALOOKUP_NONE]);
 
 Theorem grep_sem_with_numchars
-  `∀cl fls fs. consistentFS fs ⇒
-   grep_sem cl fls (fs with numchars := ns) =
-   grep_sem cl fls fs with numchars := ns`
+  `∀cl fs. consistentFS fs ⇒
+   grep_sem cl (fs with numchars := ns) =
+   grep_sem cl fs with numchars := ns`
   (recInduct grep_sem_ind
   \\ rw[grep_sem_def,add_stdo_with_numchars]
   \\ CASE_TAC \\ rw[add_stdo_with_numchars]
-  \\ rpt(pop_assum kall_tac)
+  \\ pop_assum kall_tac
+  \\ pop_assum mp_tac
+  \\ pop_assum kall_tac
   \\ qid_spec_tac`fs`
   \\ qid_spec_tac`filenames`
   \\ ho_match_mp_tac SNOC_INDUCT
@@ -776,7 +771,7 @@ Theorem grep_spec
    app (p:'ffi ffi_proj) ^(fetch_v"grep"(get_ml_prog_state()))
     [Conv NONE []]
     (STDIO fs * COMMANDLINE cl)
-    (POSTv v. &UNIT_TYPE () v * STDIO (grep_sem cl fs.files fs) * COMMANDLINE cl)`
+    (POSTv v. &UNIT_TYPE () v * STDIO (grep_sem cl fs) * COMMANDLINE cl)`
   (strip_tac
   \\ xcf"grep"(get_ml_prog_state())
   \\ xlet_auto >- (xcon \\ xsimpl)
@@ -840,11 +835,11 @@ Theorem grep_spec
   \\ xfun_spec`appthis`
      `∀f fv fs'.
       FILENAME f fv ∧ hasFreeFD fs' ∧ consistentFS fs' ∧
-      FILTER (isFile o FST) fcs = FILTER (isFile o FST) fs.inode_tbl ∧
+      FILTER (isFile o FST) fs'.inode_tbl = FILTER (isFile o FST) fs.inode_tbl ∧
       fs'.files = fs.files ⇒
       app p appthis [fv] (STDIO fs')
         (POSTv v. &UNIT_TYPE () v
-                  * STDIO (grep_sem_file (regexp_lang r) fcs f fs'))`
+                  * STDIO (grep_sem_file (regexp_lang r) f fs'))`
   >- (
     rw[]
     \\ first_x_assum match_mp_tac
@@ -853,16 +848,18 @@ Theorem grep_spec
     \\ instantiate
     \\ xsimpl
     \\ simp[grep_sem_file_def]
-    \\ `ALOOKUP fcs (File f) = ALOOKUP fs'.inode_tbl (File f)`
+    \\ `ALOOKUP fs.inode_tbl (File f) = ALOOKUP fs'.inode_tbl (File f)`
     by (
-      first_x_assum(mp_tac o Q.AP_TERM`ALOOKUP`)
+      last_x_assum(mp_tac o Q.AP_TERM`ALOOKUP`)
       \\ disch_then(mp_tac o C Q.AP_THM`File f`)
       \\ simp[ALOOKUP_FILTER,o_DEF,LAMBDA_PROD] )
     \\ fs[]
     \\ reverse IF_CASES_TAC
-    >- ( CASE_TAC \\ xsimpl \\ imp_res_tac ALOOKUP_SOME_inFS_fname )
+    >- ( CASE_TAC \\ xsimpl \\ imp_res_tac ALOOKUP_SOME_inFS_fname \\
+         fs[inFS_fname_def] >> rfs[])
+    \\ CASE_TAC >-(fs[inFS_fname_def] \\ rfs[])
     \\ imp_res_tac inFS_fname_ALOOKUP_EXISTS
-    \\ simp[]
+    \\ rfs[]
     \\ qmatch_goalsub_abbrev_tac`add_stdout _ s1`
     \\ qmatch_goalsub_abbrev_tac`_ (add_stdout _ s2) * _`
     \\ `s1 = s2` suffices_by xsimpl
@@ -909,7 +906,7 @@ Theorem grep_spec
     \\ fs[EVERY_MEM] )
   \\ first_x_assum drule
   \\ `TAKE (n+1) fls = (TAKE n fls) ++ [EL n fls]` by ( simp[TAKE_EL_SNOC] )
-  \\ simp[FOLDL_APPEND,Abbr`ff`,Abbr`fcs`]
+  \\ simp[FOLDL_APPEND,Abbr`ff`]
   \\ disch_then match_mp_tac
   \\ imp_res_tac grep_sem_file_lemma
   \\ fs[]);
@@ -917,12 +914,12 @@ Theorem grep_spec
 val st = get_ml_prog_state()
 
 Theorem grep_whole_prog_spec
-  `consistentFS ∧ ⇒ hasFreeFD fs ∧ grep_termination_assum cl ⇒
+  `consistentFS fs ⇒
    whole_prog_spec ^(fetch_v "grep" st) cl fs NONE
-     ((=) (grep_sem cl fs.files fs))`
+     ((=) (grep_sem cl fs))`
   (disch_then assume_tac
   \\ simp[whole_prog_spec_def]
-  \\ qexists_tac`grep_sem cl fs.files fs`
+  \\ qexists_tac`grep_sem cl fs`
   \\ simp[GSYM grep_sem_with_numchars,with_same_numchars]
   \\ match_mp_tac (MP_CANON (MATCH_MP app_wgframe (UNDISCH grep_spec)))
   \\ xsimpl);
